Owl/constants.v
@@ -1,5 +1,7 @@
 Record Lattice := {
   labels : Set;
+  leq : labels -> labels -> bool
+  bot : labels;
 }.
 
 Axiom L : Lattice. 
